Cambios 25/02

src/ContainersOps.dfy
@@ -1,5 +1,32 @@
 include "Ord.dfy"
 
+
+function Array2ToSeqSeq<T>(a : array2<T>, k : int) : seq<seq<T>>
+    reads a
+    requires 0 <= k <= a.Length0
+    ensures k == |Array2ToSeqSeq(a,k)|
+    ensures forall i | 0 <= i < k :: a.Length1 == |Array2ToSeqSeq(a,k)[i]|
+    ensures forall i,j | 0 <= i < k && 0 <= j < a.Length1 :: Array2ToSeqSeq(a,k)[i][j] == a[i, j]
+  {
+    if k == 0 then
+      []
+    else
+      Array2ToSeqSeq(a, k-1) + [Array2ToSeq(a, k-1, a.Length1)]
+  }
+
+  function Array2ToSeq<T>(a : array2<T>, k : int, j : int) : seq<T>
+    reads a
+    requires 0 <= k < a.Length0
+    requires 0 <= j <= a.Length1
+    ensures j == |Array2ToSeq(a,k,j)|
+    ensures forall i | 0 <= i < j :: Array2ToSeq(a,k,j)[i] == a[k, i]
+  {
+    if j == 0 then
+      []
+    else
+      Array2ToSeq(a, k, j-1) + [a[k, j-1]]
+  }
+
 /*
  *  mapSeq applies the function f to all the elements in the segment
  *  [startIdx, endIdx) of the input sequence a.
